Add many lemmas; some theorems are incomplete

ictac2021/automata.v
@@ -7,6 +7,7 @@
  *)
 
 Require Import equiv.
+Require Import Lists.List.
 
 (* Rules of RPDA A and PDA A' *)
 
@@ -61,8 +62,8 @@ Inductive ruleA'
 Definition Stack  := list (D * Theta).
 Definition Stack' := list Phi.
 
-Definition config  := Q  * Theta * Stack.
-Definition config' := Q' * Stack'.
+Definition Config  := Q  * Theta * Stack.
+Definition Config' := Q' * Stack'.
 
 Definition update_stack (u : Stack) theta com :=
   match com with
@@ -86,23 +87,37 @@ Definition update_stack' (u : Stack') com' :=
   | push' z => cons z u
   end.
 
+Definition freshness_p_on_moveA (tst : Tst) d (u : Stack) :=
+  let not_contain_d cell :=
+     match cell with (_, theta) => forall i, theta i <> d end
+  in (forall xi, tst xi <> true) ->
+     Forall not_contain_d u.
+
 Inductive moveA
-  : config -> Sigma -> D -> config -> Prop :=
+  : Config -> Sigma -> D -> Config -> Prop :=
   | MoveA :
-    forall tst asgn com q1 q2 a d z u theta theta' zth,
+    forall tst asgn com z zth u q1 q2 a d theta theta',
     ruleA q1 a tst q2 asgn com ->
     (theta, d, z) |= tst ->
     theta' = update theta asgn d ->
+    freshness_p_on_moveA tst d (cons (z, zth) u) ->
     moveA (q1, theta,  (cons (z, zth) u)) a d
           (q2, theta', update_stack (cons (z, zth) u) theta' com).
 
 Inductive moveA'
-  : config' -> Sigma -> config' -> Prop :=
+  : Config' -> Sigma -> Config' -> Prop :=
   | MoveA' :
     forall q1 q2 a z u com',
     ruleA' q1 a z q2 com' ->
     moveA' (q1, (cons z u)) a
            (q2, update_stack' (cons z u) com').
+
+Definition is_proper_stack (stack : Stack) :=
+  let is_proper_cell cell :=
+    match cell with (z, theta) => exists i, z = theta i end
+  in Forall is_proper_cell stack.
+
+(* Bisimulation relation between configs *)
 
 Inductive stack_R_stack'
   : Theta -> Stack -> Phi -> Stack' -> Prop :=
@@ -117,81 +132,791 @@ Inductive stack_R_stack'
     stack_R_stack' theta (cons (d, ptheta) u) phi (cons pphi v).
 
 Inductive config_R_config'
-  : config -> config' -> Prop :=
+  : Config -> Config' -> Prop :=
   | Config_R_config' :
     forall q theta u phi v,
     stack_R_stack' theta u phi v ->
     config_R_config' (q, theta, u) ((q, phi), v).
 
-(* Utility: sublist, proper_sublist *)
+(* freshness_p on stack *)
 
-Inductive sublist {X : Type} : list X -> list X -> Prop :=
-  | Sublist_nil    : forall l, sublist nil l
-  | Sublist_cons_right :
-      forall l1 l2 x, sublist l1 l2 -> sublist l1 (cons x l2)
-  | Sublist_cons_both :
-      forall l1 l2 x, sublist l1 l2 -> sublist (cons x l1) (cons x l2).
+Inductive Forall2 {X : Type} (P : X -> X -> Prop)
+  : list X -> Prop :=
+  | Forall2_nil : Forall2 P nil
+  | Forall2_cons x l :
+    Forall (P x) l -> Forall2 P l -> Forall2 P (x :: l).
 
-Example sublist_example_1 :
-  sublist (cons 2 (cons 3 nil)) (cons 1 (cons 2 (cons 3 nil))).
+Inductive Forall3 {X : Type} (P : X -> X -> X -> Prop)
+  : list X -> Prop :=
+  | Forall3_nil : Forall3 P nil
+  | Forall3_cons x l :
+    Forall2 (P x) l -> Forall3 P l -> Forall3 P (x :: l).
+
+Definition freshness_p_on_triple
+  (p3 p2 p1 : D * Theta) :=
+  match (p3, p2, p1) with
+    ((_, th3), (_, th2), (d, th1))
+    => freshness_p th1 d th2 th3
+  end.
+
+Definition freshness_p_on_stack theta stack :=
+  Forall3 freshness_p_on_triple ((bot, theta) :: stack).
+
+Example forall2_example_1 :
+  Forall2 le (0 :: 1 :: 3 :: 8 :: nil).
 Proof.
-  apply Sublist_cons_right.
-  apply Sublist_cons_both.
-  apply Sublist_cons_both.
-  apply Sublist_nil.
+  repeat apply Forall2_cons;
+  repeat apply Forall_cons;
+  repeat (apply le_S; try apply le_n); auto;
+  try apply Forall2_nil.
 Qed.
 
-(* Freshness on stack *)
+(* Lemmas *)
 
-Inductive freshness_on_stack
-  : Theta -> Stack -> Prop :=
-  | Freshness_on_stack :
-    forall theta stack,
-    forall u1 u2 u3 th1 th2 th3 d1 d2 d3,
-    sublist (cons (d1, th1) u1) u2 ->
-    sublist (cons (d2, th2) u2) u3 ->
-    sublist (cons (d3, th3) u3) (cons (bot, theta) stack) ->
-    freshness_p th1 d1 th2 th3 ->
-    freshness_on_stack theta stack.
+(* Forall, Forall2, Forall3 *)
 
-(* Theorems *)
+Lemma Forall_sublist {A : Type} :
+  forall p (a : A) u1 u2,
+  Forall p (u1 ++ (a :: u2)) ->
+  Forall p (u1 ++ u2).
+Proof.
+  intros p a u1 u2.
+  induction u1 as [| b u1 IHu1].
+  - (* u1 = nil -> ... *)
+  unfold app.
+  intros Hfor.
+  inversion Hfor as [| x l Hpa Hfor' [EQx EQl]].
+  exact Hfor'.
+  - (* u1 = b :: u1 -> ... *)
+  repeat rewrite<- app_comm_cons.
+  intros Hfor.
+  inversion Hfor as [| x l Hpb Hfor' [EQx EQl]].
+  clear x EQx l EQl.
+  apply Forall_cons; auto.
+Qed.
+
+Lemma Forall2_sublist {A : Type} :
+  forall p (a : A) u1 u2,
+  Forall2 p (u1 ++ (a :: u2)) ->
+  Forall2 p (u1 ++ u2).
+Proof.
+  intros p a u1 u2.
+  induction u1 as [| b u1 IHu1].
+  - (* u1 = nil -> ... *)
+  unfold app.
+  intros Hfor2.
+  inversion Hfor2 as [| x l Hfor Hfor2' [EQx EQl]].
+  exact Hfor2'.
+  - (* u1 = b :: u1 -> ... *)
+  repeat rewrite<- app_comm_cons.
+  intros Hfor2.
+  inversion Hfor2 as [| x l Hfor Hfor2' [EQx EQl]].
+  clear x EQx l EQl.
+  apply Forall2_cons.
+  + (* Forall ... *)
+  apply Forall_sublist with a; auto.
+  + (* Forall2 ... *)
+  apply IHu1; auto.
+Qed.
+
+Lemma Forall3_sublist {A : Type} :
+  forall p (a : A) u1 u2,
+  Forall3 p (u1 ++ (a :: u2)) ->
+  Forall3 p (u1 ++ u2).
+Proof.
+  intros p a u1 u2.
+  induction u1 as [| b u1 IHu1].
+  - (* u1 = nil -> ... *)
+  unfold app.
+  intros Hfor3.
+  inversion Hfor3 as [| x l Hfor2 Hfor3' [EQx EQl]].
+  exact Hfor3'.
+  - (* u1 = b :: u1 -> ... *)
+  repeat rewrite<- app_comm_cons.
+  intros Hfor3.
+  inversion Hfor3 as [| x l Hfor2 Hfor3' [EQx EQl]].
+  clear x EQx l EQl.
+  apply Forall3_cons.
+  + (* Forall ... *)
+  apply Forall2_sublist with a; auto.
+  + (* Forall2 ... *)
+  apply IHu1; auto.
+Qed.
+
+Lemma Forall2_hd2 {A : Type} :
+  forall p (a : A) b u,
+  Forall2 p (a :: b :: u) ->
+  p a b.
+Proof.
+  intros p a b u H.
+  inversion H as [| x l Hfor Hfor2 [EQx EQl]].
+  clear x EQx l EQl H Hfor2.
+  inversion Hfor as [| x l H Hfor' [EQx EQl]].
+  exact H.
+Qed.
+
+Lemma Forall3_hd3 {A : Type} :
+  forall p (a : A) b c u,
+  Forall3 p (a :: b :: c :: u) ->
+  p a b c.
+Proof.
+  intros p a b c u H.
+  inversion H as [| x l Hfor2 Hfor3' [EQx EQl]].
+  clear x EQx l EQl Hfor3' H.
+  apply Forall2_hd2 with u.
+  exact Hfor2.
+Qed.
+
+Lemma Forall2_forall_inv {A : Type} :
+  forall (p : A -> A -> Prop) u,
+  (forall b c,
+   In b u -> In c u -> p b c) ->
+  Forall2 p u.
+Proof.
+  intros p u H.
+  induction u as [| a u IHu].
+  { apply Forall2_nil. }
+  apply Forall2_cons.
+  - induction u as [| b u IHu'].
+  { apply Forall_nil. }
+  apply Forall_cons.
+  + apply H.
+  * apply in_eq.
+  * apply in_cons. apply in_eq.
+  + apply IHu'.
+  * intros b' c Hb' Hc.
+  apply H.
+  -- destruct Hb' as [EQb' | Hb''].
+  ++ rewrite<- EQb'. apply in_eq.
+  ++ apply in_cons. apply in_cons. exact Hb''.
+  -- destruct Hc as [EQc | Hc'].
+  ++ rewrite<- EQc. apply in_eq.
+  ++ apply in_cons. apply in_cons. exact Hc'.
+  * intros H'.
+  apply (Forall2_sublist _ b nil).
+  unfold app.
+  apply IHu.
+  intros b' c Hb' Hc.
+  apply H.
+  -- destruct Hb' as [EQb' | Hb''].
+  ++ rewrite<- EQb'. apply in_cons. apply in_eq.
+  ++ apply in_cons. apply in_cons. exact Hb''.
+  -- destruct Hc  as [EQc  | Hc'].
+  ++ rewrite<- EQc. apply in_cons. apply in_eq.
+  ++ apply in_cons. apply in_cons. exact Hc'.
+  - apply IHu.
+  intros b c Hb Hc.
+  apply H;
+  apply in_cons; auto.
+Qed.
+
+(* is_proper_stack *)
+
+Lemma substack_is_proper_stack :
+  forall a u1 u2,
+  is_proper_stack (u1 ++ (a :: u2)) ->
+  is_proper_stack (u1 ++ u2).
+Proof.
+  apply Forall_sublist.
+Qed.
+
+Lemma substack_is_proper_stack_1 :
+  forall a u,
+  is_proper_stack (a :: u) ->
+  is_proper_stack u.
+Proof.
+  intros a u.
+  apply (Forall_sublist _ _ nil).
+Qed.
+
+Lemma substack_is_proper_stack_2 :
+  forall a b u,
+  is_proper_stack (a :: b :: u) ->
+  is_proper_stack (a :: u).
+Proof.
+  intros a b u.
+  apply (Forall_sublist _ _ (a :: nil)).
+Qed.
+
+(* freshness_p_on_stack *)
+
+Lemma substack_keeps_freshness_p_0 :
+  forall theta d th u,
+  freshness_p_on_stack theta ((d, th) :: u) ->
+  freshness_p_on_stack th u.
+Proof.
+  intros theta d th u.
+  unfold freshness_p_on_stack.
+  intros Hfor3.
+  inversion Hfor3 as [| x l Hfor2 Hfor3' [EQx EQl]].
+  clear x l EQx EQl Hfor3.
+  inversion Hfor3' as [| x l Hfor2' Hfor3 [EQx EQl]].
+  clear x l EQx EQl Hfor3'.
+  apply Forall3_cons; auto.
+Qed.
+
+Lemma substack_keeps_freshness_p :
+  forall theta a u1 u2,
+  freshness_p_on_stack theta (u1 ++ (a :: u2)) ->
+  freshness_p_on_stack theta (u1 ++ u2).
+Proof.
+  intros theta a u1 u2.
+  unfold freshness_p_on_stack.
+  repeat rewrite app_comm_cons.
+  apply Forall3_sublist.
+Qed.
+
+Lemma substack_keeps_freshness_p_1 :
+  forall theta a u,
+  freshness_p_on_stack theta (a :: u) ->
+  freshness_p_on_stack theta u.
+Proof.
+  intros theta a u.
+  apply (substack_keeps_freshness_p _ _ nil u).
+Qed.
+
+Lemma substack_keeps_freshness_p_2 :
+  forall theta a b u,
+  freshness_p_on_stack theta (a :: b :: u) ->
+  freshness_p_on_stack theta (a :: u).
+Proof.
+  intros theta a b u.
+  apply (substack_keeps_freshness_p _ _ (a :: nil) u).
+Qed.
+
+(* freshness_p_on_moveA *)
+
+Lemma substack_keeps_freshness_p_on_moveA :
+  forall tst d a u1 u2,
+  freshness_p_on_moveA tst d (u1 ++ (a :: u2)) ->
+  freshness_p_on_moveA tst d (u1 ++ u2).
+Proof.
+  intros tst d a u1 u2.
+  unfold freshness_p_on_moveA.
+  intros Hfrs Htst.
+  assert (Hfrs' := Hfrs Htst).
+  generalize Hfrs'.
+  apply (Forall_sublist _ a).
+Qed.
+
+Lemma substack_keeps_freshness_p_on_moveA_1 :
+  forall tst d a u,
+  freshness_p_on_moveA tst d (a :: u) ->
+  freshness_p_on_moveA tst d u.
+Proof.
+  intros tst d a u.
+  apply (substack_keeps_freshness_p_on_moveA _ _ _ nil).
+Qed.
+
+Lemma substack_keeps_freshness_p_on_moveA_2 :
+  forall tst d a b u,
+  freshness_p_on_moveA tst d (a :: b :: u) ->
+  freshness_p_on_moveA tst d (a :: u).
+Proof.
+  intros tst d a b u.
+  apply (substack_keeps_freshness_p_on_moveA _ _ _ (a :: nil)).
+Qed.
+
+(* moveA *)
+
+Lemma keeping_freshness_p_when_skip :
+  forall theta zth d z u tst asgn,
+  (theta, d, z) |= tst ->
+  is_proper_stack ((z, zth) :: u) ->
+  freshness_p_on_moveA tst d ((z, zth) :: u) ->
+  forall d1 d2 th1 th2,
+  In (d1, th1) ((z, zth) :: u) ->
+  In (d2, th2) u ->
+  freshness_p_on_triple (bot, theta) (d1, th1) (d2, th2) ->
+  freshness_p_on_triple     (z, zth) (d1, th1) (d2, th2) ->
+  freshness_p_on_triple (bot, update theta asgn d) (d1, th1) (d2, th2).
+Proof.
+  intros theta zth d z u tst asgn.
+  intros Htst Hproper Hfrs_m.
+  intros d1 d2 th1 th2.
+  intros Hth1 Hth2.
+  unfold freshness_p_on_triple.
+  unfold freshness_p.
+  intros [H1 H2].
+  intros [Hz1 Hz2].
+
+  (* destruct Hfrs_m *)
+  unfold freshness_p_on_moveA in Hfrs_m.
+  destruct (tst_is_empty_or_not tst)
+  as [Htst_empty | Htst_not_empty].
+
+  - (* tst_empty -> ... *)
+  apply Hfrs_m in Htst_empty as Hfrs_m'.
+  rewrite Forall_forall in Hfrs_m'.
+  assert (Hth2' : In (d2, th2) ((z, zth) :: u)).
+  { apply in_cons. exact Hth2. }
+  assert (Hm := Hfrs_m' (d2, th2) Hth2').
+  simpl in Hm.
+
+  unfold freshness_p_on_triple.
+  unfold freshness_p.
+  split.
+  ** (* forall i j, th1 i = update ... -> ... *)
+  intros i j.
+  unfold update.
+  case (asgn j); intros EQth2.
+  +++ (* asgn j = true -> ... *)
+  apply Hm in EQth2.
+  contradiction.
+  +++ (* asgn j = false -> ... *)
+  apply H1 with j.
+  exact EQth2.
+  ** (* forall j, d1 = update ... -> ... *)
+  intros j.
+  unfold update.
+  case (asgn j); intros EQd2.
+  +++ (* asgn j = true -> ... *)
+  (* destruct Hproper *)
+  unfold is_proper_stack in Hproper.
+  rewrite Forall_forall in Hproper.
+  assert (Hprop2 := Hproper (d2, th2) Hth2').
+  simpl in Hprop2.
+  destruct Hprop2 as [i2 Hprop2].
+  rewrite EQd2 in Hprop2.
+  symmetry in Hprop2.
+  apply Hm in Hprop2.
+  contradiction.
+  +++ (* asgn j = false -> ... *)
+  apply H2 with j.
+  exact EQd2.
+
+  - (* tst_not_empty -> ... *)
+  clear Hfrs_m.
+  unfold models in Htst.
+  unfold Theta_D_D_models_Tst in Htst.
+  destruct Htst as [Htst' Htst_top].
+  destruct Htst_not_empty as [xi Htst_true].
+  case_eq xi.
+  ** (* xi = inl n -> ... *)
+  intros n EQxi.
+  rewrite EQxi in Htst_true.
+  rewrite<- Htst' in Htst_true.
+  clear xi EQxi.
+
+  split.
+  --- (* forall i j, th1 i = update ... -> ... *)
+  intros i j.
+  unfold update.
+  case (asgn j); intros EQth2.
+  +++ (* asgn j = true -> ... *)
+  apply H1 with n.
+  rewrite Htst_true.
+  exact EQth2.
+  +++ (* asgn j = false -> ... *)
+  apply H1 with j.
+  exact EQth2.
+  --- (* forall j, d1 = update ... -> ... *)
+  intros j.
+  unfold update.
+  case (asgn j); intros EQd2.
+  +++ (* asgn j = true -> ... *)
+  apply H2 with n.
+  rewrite Htst_true.
+  exact EQd2.
+  +++ (* asgn j = false -> ... *)
+  apply H2 with j.
+  exact EQd2.
+
+  ** (* xi = inr top -> ... *)
+  intros t EQxi.
+  destruct t.
+  rewrite EQxi in Htst_true.
+  rewrite<- Htst_top in Htst_true.
+  clear xi EQxi.
+
+  (* destruct Hproper *)
+  unfold is_proper_stack in Hproper.
+  rewrite Forall_forall in Hproper.
+  assert (Hzth: In (z, zth) ((z, zth) :: u)).
+  { apply in_eq. }
+  assert (Hpropz := Hproper (z, zth) Hzth).
+  simpl in Hpropz.
+  destruct Hpropz as [iz Hpropz].
+
+  split.
+  --- (* forall i j, th1 i = update ... -> ... *)
+  intros i j.
+  unfold update.
+  case (asgn j); intros EQth2.
+  +++ (* asgn j = true -> ... *)
+  apply Hz1 with iz.
+  rewrite EQth2.
+  rewrite<- Htst_true.
+  apply Hpropz.
+  +++ (* asgn j = false -> ... *)
+  apply H1 with j.
+  exact EQth2.
+  --- (* forall j, d1 = update ... -> ... *)
+  intros j.
+  unfold update.
+  case (asgn j); intros EQd2.
+  +++ (* asgn j = true -> ... *)
+  apply Hz2 with iz.
+  rewrite EQd2.
+  rewrite<- Htst_true.
+  apply Hpropz.
+  +++ (* asgn j = false -> ... *)
+  apply H2 with j.
+  exact EQd2.
+Qed.
+
+Lemma moveA_keeps_freshness_p_when_skip :
+  forall theta zth d z u tst asgn,
+  (theta, d, z) |= tst ->
+  is_proper_stack ((z, zth) :: u) ->
+  freshness_p_on_moveA tst d ((z, zth) :: u) ->
+  freshness_p_on_stack theta ((z, zth) :: u) ->
+  freshness_p_on_stack (update theta asgn d) ((z, zth) :: u).
+Proof.
+  intros theta zth d z u tst asgn.
+  intros Htst Hproper Hfrs_m Hfrs_s.
+  unfold freshness_p_on_stack.
+  unfold freshness_p_on_stack in Hfrs_s.
+  apply Forall3_cons.
+  - (* Forall2 ... ((z, zth) :: u) *)
+  apply Forall2_cons.
+  + (* Forall ... u *)
+  apply Forall_forall.
+  intros [d1 th1] H1.
+  (* freshness_p_on_triple (, update ...) (z, zth) (d1, th1) *)
+  apply (keeping_freshness_p_when_skip _ zth _ z u tst asgn); auto.
+  * (* In (z, zth) ((z, zth) :: u) *)
+  apply in_eq.
+  * (* freshness_p_on_triple (, theta) (z, zth) (d1, th1) *)
+  inversion Hfrs_s as [| x1 l1 Hfor2 Hfor3 [EQx1 EQl1]].
+  clear x1 EQx1 l1 EQl1 Hfor3.
+  inversion Hfor2 as [| x1 l1 Hfor Hfor2' [EQx1 EQl1]].
+  clear x1 EQx1 l1 EQl1 Hfor2 Hfor2'.
+  rewrite Forall_forall in Hfor.
+  apply Hfor.
+  exact H1.
+  * (* freshness_p_on_triple (z, zth) (z, zth) (d1, th) *)
+  unfold freshness_p_on_triple.
+  unfold freshness_p.
+  split.
+  -- intros i j Hth1. exists j; auto.
+  -- intros j Hd1. exists j; auto.
+
+  + (* Forall2 ... u *)
+  induction u as [| [d1 th1] u IHu].
+  { apply Forall2_nil. }
+  apply Forall2_cons.
+  * (* Forall ... u *)
+  apply Forall_forall.
+  intros [d2 th2] H2.
+  (* freshness_p_on_triple (, update ...) (d1, th1) (d2, th2) *)
+  apply (keeping_freshness_p_when_skip _ zth _ z ((d1, th1) :: u) tst asgn);
+  auto.
+  -- apply in_cons. apply in_eq.
+  -- apply in_cons. exact H2.
+  -- (* freshness_p_on_triple (, theta) (d1, th1) (d2, th2) *)
+  inversion Hfrs_s as [| x1 l1 Hfor2 Hfor3 [EQx1 EQl1]].
+  clear x1 EQx1 l1 EQl1 Hfor3.
+  inversion Hfor2 as [| x1 l1 Hfor Hfor2' [EQx1 EQl1]].
+  clear x1 EQx1 l1 EQl1 Hfor2 Hfor.
+  inversion Hfor2' as [| x1 l1 Hfor Hfor2 [EQx1 EQl1]].
+  clear x1 EQx1 l1 EQl1 Hfor2 Hfor2'.
+  rewrite Forall_forall in Hfor.
+  apply Hfor.
+  exact H2.
+  -- (* freshness_p_on_triple (z, zth) (d1, th1) (d2, th2) *)
+  inversion Hfrs_s as [| x1 l1 Hfor2 Hfor3 [EQx1 EQl1]].
+  clear x1 EQx1 l1 EQl1 Hfor2.
+  inversion Hfor3 as [| x1 l1 Hfor2 Hfor3' [EQx1 EQl1]].
+  clear x1 EQx1 l1 EQl1 Hfor3 Hfor3'.
+  inversion Hfor2 as [| x1 l1 Hfor Hfor2' [EQx1 EQl1]].
+  clear x1 EQx1 l1 EQl1 Hfor2 Hfor2'.
+  rewrite Forall_forall in Hfor.
+  apply Hfor.
+  exact H2.
+
+  * (* Forall2 ... u *)
+  apply IHu.
+  -- apply (substack_is_proper_stack (d1, th1) ((z, zth) :: nil)); auto.
+  -- apply (substack_keeps_freshness_p_on_moveA _ _ (d1,th1) ((z,zth)::nil));
+     auto.
+  -- apply (Forall3_sublist _ (d1, th1) ((bot,theta)::(z,zth)::nil)); auto.
+
+  - (* Forall3 ... ((z, zth) :: u) *)
+  apply (Forall3_sublist _ (bot, theta) nil); auto.
+Qed.
+
 
 Lemma moveA_inversion :
   forall q q' theta theta' u u' a d,
   moveA (q, theta, u) a d (q', theta', u') ->
-  exists tst asgn com,
+  exists tst asgn com z zth uu,
   ruleA q a tst q' asgn com /\
+  u = cons (z, zth) uu /\
+  (theta, d, z) |= tst /\
   theta' = update theta asgn d /\
-  u' = update_stack u theta' com.
+  u' = update_stack u theta' com /\
+  freshness_p_on_moveA tst d u.
 Proof.
   intros q q' theta theta' u u' a d.
   intros Hm.
-  inversion Hm as [tst asgn com].
-  exists tst, asgn, com.
+  inversion Hm as [tst asgn com z zth uu].
+  exists tst, asgn, com, z, zth, uu.
   split; [| split]; auto.
 Qed.
 
-Lemma bisimilar_1 :
-  forall q theta_n phi_n v u,
-  forall a d q' theta' v',
-  config_R_config' (q, theta_n, v) ((q, phi_n), u) ->
-  moveA (q, theta_n, v) a d (q', theta', v') ->
-  exists phi'' u',
-  moveA' ((q, phi_n), u) a ((q', phi''), u') /\
-  config_R_config' (q', theta', v') ((q', phi''), u').
+Lemma no_moveA_on_nil :
+  forall q q' theta theta' a d v',
+  ~ moveA (q, theta, nil) a d (q', theta', v').
 Proof.
-  intros q theta_n phi_n v u.
-  intros a d q' theta' v'.
-  intros HR HmA.
+  intros q q' theta theta' a d v'.
+  intro H.
+  inversion H.
+Qed.
+
+Lemma config_R_nil_nil_1 :
+  forall q theta u phi,
+  config_R_config' (q, theta, u) (q, phi, nil) ->
+  u = nil.
+Proof.
+  intros q theta u phi.
+  intro H.
+  inversion H as [q1 theta1 u1 phi1 v1 HR].
+  inversion HR.
+  reflexivity.
+Qed.
+
+Lemma config_R_nil_nil_2 :
+  forall q theta v phi,
+  config_R_config' (q, theta, nil) (q, phi, v) ->
+  v = nil.
+Proof.
+  intros q theta v phi.
+  intro H.
+  inversion H as [q1 theta1 u1 phi1 v1 HR].
+  inversion HR.
+  reflexivity.
+Qed.
+
+Lemma moveA_keeps_proper_stack :
+  forall q theta u a d q' theta' u',
+  moveA (q, theta, u) a d (q', theta', u') ->
+  is_proper_stack u ->
+  is_proper_stack u'.
+Proof.
+  intros q theta u a d q' theta' u'.
+  intros HmA Hproper.
   apply moveA_inversion in HmA as HrA.
-  destruct HrA as [tst [asgn [com [HrA [Hth' Hv']]]]].
-  case_eq u.
+  destruct HrA
+  as [tst [asgn [com [z [zth [uu [HrA [Hu [Htst [Hth' [Hu' Hfrs_u]]]]]]]]]]].
+  case_eq com;
+  [intros Hcom | intros Hcom | intros j Hcom];
+  rewrite Hcom in Hu';
+  rewrite Hcom in HrA;
+  clear com Hcom;
+  rewrite Hu in Hu';
+  unfold update_stack in Hu'.
+  - (* com = pop -> ... *)
+  rewrite<- Hu' in Hu.
+  clear uu Hu'.
+  unfold is_proper_stack.
+  unfold is_proper_stack in Hproper.
+  rewrite Hu in Hproper.
+  inversion Hproper as [| x l Hcell Hproper_u' [EQx EQl]].
+  apply Hproper_u'.
+  - (* com = skip -> ... *)
+  rewrite<- Hu' in Hu.
+  clear uu Hu'.
+  rewrite<- Hu.
+  exact Hproper.
+  - (* com = push -> ... *)
+  rewrite Hu'.
+  unfold is_proper_stack.
+  apply Forall_cons.
+  { exists j; reflexivity. }
+  rewrite<- Hu.
+  unfold is_proper_stack in Hproper.
+  exact Hproper.
+Qed.
+
+Lemma moveA_keeps_freshness_p :
+  forall q theta u a d q' theta' u',
+  moveA (q, theta, u) a d (q', theta', u') ->
+  freshness_p_on_stack theta u ->
+  freshness_p_on_stack theta' u'.
+Proof.
+  intros q theta u a d q' theta' u'.
+  intros HmA Hfresh.
+  apply moveA_inversion in HmA as HrA.
+  destruct HrA
+  as [tst [asgn [com [z [zth [uu [HrA [Hu [Htst [Hth' [Hu' Hfrs_u]]]]]]]]]]].
+  case_eq com;
+  [intros Hcom | intros Hcom | intros j Hcom];
+  rewrite Hcom in Hu';
+  rewrite Hcom in HrA;
+  clear com Hcom;
+  rewrite Hu in Hu';
+  unfold update_stack in Hu'.
+  - (* com = pop -> ... *)
+  rewrite<- Hu' in Hu.
+  clear uu Hu'.
+  inversion Hfresh as [|x l Hfor2 Hfor3 [EQx EQl]].
+  clear x EQx l EQl.
+  unfold freshness_p_on_stack.
+  apply Forall3_cons.
+  + (* Forall2 ... *)
+  case_eq u'.
+  { intros. apply Forall2_nil. }
+  intros p l EQu'.
+  unfold freshness_p_on_moveA in Hfrs_u.
+  unfold freshness_p.
+
+
 Admitted.
-(*
+
+(* Theorem on bisimilarity *)
+
+Lemma bisimilar_1 :
+  forall q theta_n phi_n u v,
+  forall a d q' theta' u',
+    moveA (q, theta_n, u) a d (q', theta', u') ->
+    config_R_config' (q, theta_n, u) ((q, phi_n), v) ->
+    freshness_p_on_stack theta_n u ->
+    is_proper_stack u ->
+    is_equiv_rel phi_n -> Forall is_equiv_rel v ->
+  exists phi'' v',
+    moveA' ((q, phi_n), v) a ((q', phi''), v') /\
+    config_R_config' (q', theta', u') ((q', phi''), v').
+Proof.
+  intros q theta_n phi_n u v.
+  intros a d q' theta' u'.
+  intros HmA HR.
+  intros Hfresh Hproper Heq_phi_n Heq_v.
+  apply moveA_inversion in HmA as HrA.
+  destruct HrA
+  as [tst [asgn [com [z [zth [uu [HrA [Hu [Htst [Hth' [Hu' Hfrs_u]]]]]]]]]]].
+  case_eq v.
+  { (* v = nil -> ... *)
+  intro Hv.
+  rewrite Hv in HR.
+  apply config_R_nil_nil_1 in HR as Hu_nil.
+  rewrite Hu_nil in HmA.
+  apply no_moveA_on_nil in HmA.
+  contradiction.
+  }
+  (* v = phi :: vv -> ... *)
+  intros phi1 vv Hv.
+
+  inversion HR as [q1 theta1 u1 phi' v1 HsR [EQq1 EQth1 EQu1] [EQphi' EQv1]].
+  clear q1 EQq1 theta1 EQth1 u1 EQu1;
+  clear phi' EQphi' v1 EQv1.
+  inversion HsR
+  as [theta2 phi'2 Hbot Hth2 Hu_nil |
+      theta2 theta3 d1 phi' phi2 u1 v1 Hphi_n HsR1 EQth2 EQu1 EQphi' EQv1].
+  { (* nil = u -> ... *)
+  rewrite Hu in Hu_nil;
+  discriminate Hu_nil.
+  }
+  (* ((d1, theta3) :: u1) = u *)
+  clear theta2 EQth2 phi' EQphi'.
+  rewrite Hu in EQu1.
+  injection EQu1; clear EQu1.
+  intros EQu1 EQth3 EQd1.
+  rewrite EQu1 in HsR1; clear u1 EQu1.
+  rewrite EQd1 in Hphi_n; clear d1 EQd1.
+  rewrite<- EQth3 in Hu; clear zth EQth3.
+  rewrite Hv in EQv1.
+  injection EQv1; clear EQv1.
+  intros EQv1 EQphi2.
+  rewrite EQv1 in HsR1; clear v1 EQv1.
+  rewrite EQphi2 in HsR1; clear phi2 EQphi2.
+
   case_eq com.
-  - intros Hcom.
+  - (* com = pop -> ... *)
+  intros Hcom.
+  rewrite Hcom in Hu'.
   rewrite Hcom in HrA.
-  apply (ruleA'_pop q phi_n a _ q' (composition (composition phi_n)) tst asgn) in HrA.
-  rewrite Hcom in Hv'.
-  unfold update_stack in Hv'.
-  *)
+  clear com Hcom.
+  assert (HtstHth' := conj Htst Hth').
+  apply ex_intro with (x := d) in HtstHth' .
+  apply meanings_of_Phi_tst_asgn in HtstHth'.
+  destruct HtstHth' as [phi3 [_ [Hphitst Hthphi]]].
+  exists (composition (composition phi1 phi_n) phi3).
+  exists (update_stack' v pop').
+  rewrite Hv.
+  split.
+  + (* moveA' ... *)
+  apply MoveA'.
+  apply ruleA'_pop with (tst := tst) (asgn := asgn);
+  auto.
+  * (* composable phi1 phi_n *)
+  inversion HsR1
+  as [theta2 phi'2 Hbot EQth2 EQuu EQphi'2 EQvv |
+     theta1' theta2 d1 phi_n' phi2 uu1 vv1 Hthphi1' HsR2 EQth1' EQuu EQphi_n' EQvv].
+  -- (* nil = vv -> ... *)
+  apply (double_models_means_composable theta_bot theta3 theta_n bot z).
+  auto.
+  -- (* (phi2 :: vv1) = vv -> ... *)
+  apply (double_models_means_composable theta2 theta3 theta_n d1 z).
+  auto.
+  * (* composableT phi_n phi3 *)
+  apply (double_models_means_composableT theta3 theta_n theta' z).
+  auto.
+
+  + (* config_R_config' ... *)
+  rewrite Hu in Hu'.
+  unfold update_stack in Hu'.
+  rewrite Hu'.
+  rewrite Hu' in HmA.
+  clear u' Hu'.
+
+  unfold update_stack'.
+  apply Config_R_config'.
+
+  case_eq vv.
+  * (* vv = nil -> ... *)
+  intros EQvv.
+  rewrite EQvv in HsR1.
+  rewrite EQvv in Hv.
+  clear vv EQvv.
+  inversion HsR1
+  as [theta2 phi'2 Hbot EQth2 EQuu EQphi'2 EQvv |].
+  clear theta2 EQth2 phi'2 EQphi'2 EQvv.
+  rewrite<- EQuu in Hu.
+  rewrite<- EQuu in HsR1.
+  rewrite<- EQuu in HmA.
+  clear uu EQuu.
+
+  unfold freshness_p_on_moveA in Hfrs_u.
+
+  apply Stack_R_stack'_nil.
+  apply (meanings_of_composition theta_bot theta_n theta' bot z).
+  -- (* is_equiv_rel (composition phi1 phi_n) *)
+  apply composition_is_equiv_rel.
+  ++ split; auto.
+  rewrite Hv in Heq_v.
+  inversion Heq_v.
+  auto.
+  ++ apply (double_models_means_composable theta_bot theta3 theta_n bot z).
+  auto.
+  -- (* freshness_p theta_bot bot theta_n theta' *)
+  unfold freshness_p.
+  split.
+  ++ intros i j.
+  rewrite Hth'.
+  unfold update.
+  case_eq (asgn j).
+  ** intros Hasgn Hbot_d.
+
+
+(*
+inversion Hfresh as [th0 u0 Hf EQth0 EQu0].
+clear th0 EQth0 u0 EQu0.
+
+
+
+sublist ((d2, theta_n))
+sublist ((d3, theta') :: u3) ((bot, theta_n) :: u)
+freshness_p theta_bot bot theta_n theta'
+*)
+  Admitted.
